src/Crypto/AESEncryption.dfy
@@ -25,7 +25,7 @@ module {:extern "AESEncryption"} AESEncryption {
   predicate {:axiom} EncryptionOutputEncryptedWithAAD(ciphertext: EncryptionOutput, aad: seq<uint8>)
   predicate {:axiom} CiphertextGeneratedWithPlaintext (ciphertext: seq<uint8>, plaintext: seq<uint8>)
   predicate {:axiom} EncryptedWithKey(ciphertext: seq<uint8>, key: seq<uint8>)
-  predicate {:axiom} DecryptedWithKey(plaintext: seq<uint8>, key: seq<uint8>)
+  predicate {:axiom} DecryptedWithKey(key: seq<uint8>, plaintext: seq<uint8>)
 
   function method EncryptionOutputFromByteSeq(s: seq<uint8>, encAlg: EncryptionSuites.EncryptionSuite): (encArt: EncryptionOutput)
     requires encAlg.Valid()
@@ -79,7 +79,7 @@ module {:extern "AESEncryption"} AESEncryption {
     requires |authTag| == encAlg.tagLen as int
     ensures res.Success? ==> PlaintextDecryptedWithAAD(res.value, aad)
     ensures res.Success? ==> CiphertextGeneratedWithPlaintext(cipherTxt, res.value)
-    ensures res.Success? ==> DecryptedWithKey(res.value, key)
+    ensures res.Success? ==> DecryptedWithKey(key, res.value)
 
   method AESDecrypt(encAlg: EncryptionSuites.EncryptionSuite, key: seq<uint8>, cipherTxt: seq<uint8>, authTag: seq<uint8>, iv: seq<uint8>, aad: seq<uint8>)
       returns (res: Result<seq<uint8>>)
@@ -92,7 +92,7 @@ module {:extern "AESEncryption"} AESEncryption {
     ensures res.Success? ==> |res.value| == |cipherTxt|
     ensures res.Success? ==> PlaintextDecryptedWithAAD(res.value, aad)
     ensures res.Success? ==> CiphertextGeneratedWithPlaintext(cipherTxt, res.value)
-    ensures res.Success? ==> DecryptedWithKey(res.value, key)
+    ensures res.Success? ==> DecryptedWithKey(key, res.value)
     {
       res := AESDecryptExtern(encAlg, key, cipherTxt, authTag, iv, aad);
       if (res.Success? && |cipherTxt| != |res.value|){
